Clean up fe25519_word64ize, give examples
As per
https://github.com/mit-plv/fiat-crypto/commit/dc8a141d13984bc39cf7523856b678a48428dbcc#commitcomment-19672297

Previously, the proofs were not unfolding the boolean comparisons that
eliminate opaque proofs from the resulting proof term.  We have to jump
through a number of hoops because Coq is really bad at dealing with big
terms, and so since we can't unfold all of the identifiers early, we
unfold some of them and alias other ones, so that we can unfold the
right ones with a hopefully-not-too-long cbv list at the end.  (This
would be a lot prettier if wish #4473
(https://coq.inria.fr/bugs/show_bug.cgi?id=4473) were granted.)

src/Specific/GF25519BoundedCommon.v
@@ -253,7 +253,7 @@ Definition word31_to_unbounded_word (x : word 31) : unbounded_word 31.
 Proof. apply (word_to_unbounded_word x); reflexivity. Defined.
 
 Local Opaque word64.
-Declare Reduction app_tuple_map := cbv [app_wire_digitsW app_fe25519W app_fe25519 HList.mapt HList.mapt' Tuple.map on_tuple List.map List.app length_fe25519 List.length wire_widths Tuple.from_list Tuple.from_list' Tuple.to_list Tuple.to_list' word64ize fst snd].
+Declare Reduction app_tuple_map := cbv [app_wire_digitsW app_fe25519W app_fe25519 HList.mapt HList.mapt' Tuple.map on_tuple List.map List.app length_fe25519 List.length wire_widths Tuple.from_list Tuple.from_list' Tuple.to_list Tuple.to_list' fst snd].
 Definition fe25519WToZ (x : fe25519W) : Specific.GF25519.fe25519
   := Eval app_tuple_map in
       app_fe25519W x (Tuple.map (fun v : word64 => v : Z)).
@@ -475,12 +475,37 @@ Proof.
   reflexivity.
 Qed.
 
+Module opt.
+  Definition word64ToZ := Eval vm_compute in word64ToZ.
+  Definition word64ToN := Eval vm_compute in @wordToN bit_width.
+  Definition NToWord64 := Eval vm_compute in NToWord64.
+  Definition bit_width := Eval vm_compute in bit_width.
+  Definition Zleb := Eval cbv [Z.leb] in Z.leb.
+  Definition andb := Eval vm_compute in andb.
+  Definition word64ize := Eval vm_compute in word64ize.
+End opt.
+
+Local Transparent bit_width.
+Local Ltac do_change lem :=
+  match lem with
+  | context L[andb (?x <=? ?y)%Z (?y <=? ?z)]
+    => let x' := (eval vm_compute in x) in
+       let z' := (eval vm_compute in z) in
+       lazymatch y with
+       | word64ToZ (word64ize ?v)
+         => let y' := constr:(opt.word64ToZ (opt.word64ize v)) in
+            let L' := context L[andb (opt.Zleb x' y') (opt.Zleb y' z')] in
+            do_change L'
+       end
+  | _ => lem
+  end.
 Definition fe25519_word64ize (x : fe25519) : fe25519.
 Proof.
   set (x' := x).
   hnf in x; destruct_head' prod.
   let lem := constr:(exist_fe25519W (fe25519W_word64ize (proj1_fe25519W x'))) in
-  let lem := (eval cbv [proj1_fe25519W x' fe25519W_word64ize proj_word exist_fe25519W Build_bounded_word Build_bounded_word'] in lem) in
+  let lem := (eval cbv [proj1_fe25519W x' fe25519W_word64ize proj_word exist_fe25519W Build_bounded_word' Build_bounded_word] in lem) in
+  let lem := do_change lem in
   refine (lem _);
     change (is_bounded (fe25519WToZ (fe25519W_word64ize (proj1_fe25519W x'))) = true);
     abstract (rewrite fe25519W_word64ize_id; apply is_bounded_proj1_fe25519).
@@ -491,6 +516,8 @@ Proof.
   hnf in x; destruct_head' prod.
   let lem := constr:(exist_wire_digitsW (wire_digitsW_word64ize (proj1_wire_digitsW x'))) in
   let lem := (eval cbv [proj1_wire_digitsW x' wire_digitsW_word64ize proj_word exist_wire_digitsW Build_bounded_word Build_bounded_word'] in lem) in
+  let lem := do_change lem in
+  let lem := (eval cbv [word64ize opt.word64ize andb Z.leb Z.compare CompOpp Pos.compare] in lem) in
   refine (lem _);
     change (wire_digits_is_bounded (wire_digitsWToZ (wire_digitsW_word64ize (proj1_wire_digitsW x'))) = true);
     abstract (rewrite wire_digitsW_word64ize_id; apply is_bounded_proj1_wire_digits).
@@ -500,9 +527,11 @@ Defined.
 
 (* Precompute constants *)
 
-Definition one := Eval vm_compute in exist_fe25519 Specific.GF25519.one_ eq_refl.
+Definition one' := Eval vm_compute in exist_fe25519 Specific.GF25519.one_ eq_refl.
+Definition one := Eval cbv [one' fe25519_word64ize word64ize andb opt.word64ToZ opt.word64ize opt.Zleb Z.compare CompOpp Pos.compare Pos.compare_cont] in fe25519_word64ize one'.
 
-Definition zero := Eval vm_compute in exist_fe25519 Specific.GF25519.zero_ eq_refl.
+Definition zero' := Eval vm_compute in exist_fe25519 Specific.GF25519.zero_ eq_refl.
+Definition zero := Eval cbv [zero' fe25519_word64ize word64ize andb opt.word64ToZ opt.word64ize opt.Zleb Z.compare CompOpp Pos.compare Pos.compare_cont] in fe25519_word64ize zero'.
 
 Lemma fold_chain_opt_gen {A B} (F : A -> B) is_bounded ls id' op' id op chain
       (Hid_bounded : is_bounded (F id') = true)
